Fixed Teleport.thy

thys/Registers/QHoare.thy
@@ -4,33 +4,37 @@ theory QHoare
   imports Quantum_Extra
 begin
 
-no_notation Order.top ("\<top>\<index>")
-
 locale qhoare =
   fixes memory_type :: "'mem itself"
 begin
 
-definition "apply U R = R U" for R :: \<open>'a update \<Rightarrow> 'mem update\<close>
-definition "ifthen R x = R (butterket x x)" for R :: \<open>'a update \<Rightarrow> 'mem update\<close>
-definition "program S = fold (o\<^sub>C\<^sub>L) S id_cblinfun" for S :: \<open>'mem update list\<close>
+type_synonym 'm statement = \<open>'m update list\<close>
+type_synonym 'm program = \<open>'m statement list\<close>
 
+definition \<open>seq P Q = [q o\<^sub>C\<^sub>L p. p \<leftarrow> P, q \<leftarrow> Q]\<close> for P Q :: \<open>'mem statement\<close>
+definition \<open>program S = foldr seq S [id_cblinfun]\<close> for S :: \<open>'mem program\<close>
+definition \<open>apply U R = [R U]\<close> for R :: \<open>'a update \<Rightarrow> 'mem update\<close>
+definition \<open>ifthenelse R M P Q = seq [R (Proj (ccspan (ket ` M)))] (program P) @
+                                 seq [R (Proj (ccspan (ket ` (-M))))] (program Q)\<close>
+  for R :: \<open>'a update \<Rightarrow> 'mem update\<close> and P Q :: \<open>'mem program\<close>
 
-definition hoare :: \<open>'mem ell2 ccsubspace \<Rightarrow> ('mem ell2 \<Rightarrow>\<^sub>C\<^sub>L 'mem ell2) list \<Rightarrow> 'mem ell2 ccsubspace \<Rightarrow> bool\<close> where
-  "hoare C p D \<longleftrightarrow> (\<forall>\<psi>\<in>space_as_set C. program p *\<^sub>V \<psi> \<in> space_as_set D)" for C p D
+definition hoare :: \<open>'mem ell2 ccsubspace \<Rightarrow> 'mem program \<Rightarrow> 'mem ell2 ccsubspace \<Rightarrow> bool\<close> where
+  \<open>hoare C p D \<longleftrightarrow> (\<forall>\<psi> \<in> space_as_set C. \<forall>A \<in> set (program p). A *\<^sub>V \<psi> \<in> space_as_set D)\<close> for C p D
 
-definition EQ :: "('a update \<Rightarrow> 'mem update) \<Rightarrow> 'a ell2 \<Rightarrow> 'mem ell2 ccsubspace" (infix "=\<^sub>q" 75) where
-  "EQ R \<psi> = R (selfbutter \<psi>) *\<^sub>S \<top>"
+definition EQ :: \<open>('a update \<Rightarrow> 'mem update) \<Rightarrow> 'a ell2 \<Rightarrow> 'mem ell2 ccsubspace\<close> (infix "=\<^sub>q" 75) where
+  \<open>EQ R \<psi> = R (proj \<psi>) *\<^sub>S \<top>\<close>
 
-lemma program_skip[simp]: "program [] = id_cblinfun"
-  by (simp add: qhoare.program_def)
+lemma seq_assoc: \<open>seq (seq P Q) R = seq P (seq Q R)\<close>
+  apply (induction P)
+  by (simp_all add: map_concat o_def seq_def cblinfun_compose_assoc)
 
-lemma program_seq: "program (p1@p2) = program p2 o\<^sub>C\<^sub>L program p1"
-  apply (induction p2 rule:rev_induct)
-   apply (simp_all add: program_def)
-  by (meson cblinfun_assoc_left(1))
+lemma program_seq: \<open>program (p1@p2) = seq (program p1) (program p2)\<close>
+  apply (induction p1)
+   apply (simp add: program_def seq_def)
+  by (simp add: program_def seq_assoc)
 
-lemma hoare_seq[trans]: "hoare C p1 D \<Longrightarrow> hoare D p2 E \<Longrightarrow> hoare C (p1@p2) E"
-  by (auto simp: program_seq hoare_def)
+lemma hoare_seq[trans]: \<open>hoare C p1 D \<Longrightarrow> hoare D p2 E \<Longrightarrow> hoare C (p1@p2) E\<close>
+  by (auto simp: program_seq hoare_def seq_def)
 
 lemma hoare_weaken_left[trans]: \<open>A \<le> B \<Longrightarrow> hoare B p C \<Longrightarrow> hoare A p C\<close>
   unfolding hoare_def
@@ -40,23 +44,22 @@ lemma hoare_weaken_right[trans]: \<open>hoare A p B \<Longrightarrow> B \<le> C 
   unfolding hoare_def 
   by (meson in_mono less_eq_ccsubspace.rep_eq) 
 
-lemma hoare_skip: "C \<le> D \<Longrightarrow> hoare C [] D"
+lemma hoare_skip: \<open>C \<le> D \<Longrightarrow> hoare C [] D\<close>
   by (auto simp: program_def hoare_def in_mono less_eq_ccsubspace.rep_eq)
 
 lemma hoare_apply: 
-  assumes "R U *\<^sub>S pre \<le> post"
-  shows "hoare pre [apply U R] post"
-  using assms 
-  apply (auto simp: hoare_def program_def apply_def)
+  assumes \<open>R U *\<^sub>S pre \<le> post\<close>
+  shows \<open>hoare pre [apply U R] post\<close>
+  using assms apply (auto simp: hoare_def program_def apply_def seq_def)
   by (metis (no_types, lifting) cblinfun_image.rep_eq closure_subset imageI less_eq_ccsubspace.rep_eq subsetD)
 
-lemma hoare_ifthen: 
+lemma hoare_ifthenelse:
   fixes R :: \<open>'a update \<Rightarrow> 'mem update\<close>
-  assumes "R (selfbutter (ket x)) *\<^sub>S pre \<le> post"
-  shows "hoare pre [ifthen R x] post"
-  using assms 
-  apply (auto simp: hoare_def program_def ifthen_def butterfly_def)
-  by (metis (no_types, lifting) cblinfun_image.rep_eq closure_subset imageI less_eq_ccsubspace.rep_eq subsetD)
+  assumes \<open>hoare (R (Proj (ccspan (ket ` M))) *\<^sub>S pre) P post\<close>
+  assumes \<open>hoare (R (Proj (ccspan (ket ` (-M)))) *\<^sub>S pre) Q post\<close>
+  shows \<open>hoare pre [ifthenelse R M P Q] post\<close>
+  using assms
+  by (auto simp: program_def[of \<open>[_]\<close>] hoare_def ifthenelse_def butterfly_def seq_def cblinfun_apply_in_image')
 
 end
 
